Foundation/Modal/Kripke/AxiomWeakPoint2.lean
@@ -1,19 +1,31 @@
 import Foundation.Modal.Kripke.Completeness
+import Foundation.Vorspiel.HRel.Convergent
 
 
 namespace LO.Modal
 
 namespace Kripke
 
-open Formula.Kripke
-
-instance : IsWeakConfluent _ whitepoint.Rel := ⟨by tauto⟩
-
-section definability
 
 variable {F : Kripke.Frame}
 
-lemma validate_WeakPoint2_of_weakConfluent [IsWeakConfluent _ F] : F ⊧ (Axioms.WeakPoint2 (.atom 0) (.atom 1)) := by
+namespace Frame
+
+class IsPiecewiseConvergent (F : Frame) extends _root_.IsPiecewiseConvergent F.Rel
+
+end Frame
+
+
+instance : whitepoint.IsPiecewiseConvergent where
+  p_convergent := by tauto
+
+
+section definability
+
+open Formula (atom)
+open Formula.Kripke
+
+lemma validate_WeakPoint2_of_weakConfluent [F.IsPiecewiseConvergent] : F ⊧ (Axioms.WeakPoint2 (.atom 0) (.atom 1)) := by
   rintro V x;
   apply Satisfies.imp_def.mpr;
   suffices
@@ -26,25 +38,27 @@ lemma validate_WeakPoint2_of_weakConfluent [IsWeakConfluent _ F] : F ⊧ (Axioms
     by_contra hC;
     subst hC;
     contradiction;
-  obtain ⟨u, Ryu, Rzu⟩ := IsWeakConfluent.weak_confluent ⟨Rxy, Rxz, nyz⟩;
+  obtain ⟨u, Ryu, Rzu⟩ := IsPiecewiseConvergent.p_convergent Rxy Rxz nyz;
   have : V u 0 := h₁ _ Ryu;
   have : ¬V u 0 := h₂ _ Rzu;
   contradiction;
 
-lemma weakConfluent_of_validate_WeakPoint2 : F ⊧ (Axioms.WeakPoint2 (.atom 0) (.atom 1)) → WeakConfluent F := by
-  contrapose;
-  intro hCon;
-  obtain ⟨x, y, Rxy, z, Rxz, nyz, hu⟩ := by simpa [WeakConfluent] using hCon;
-  apply ValidOnFrame.not_of_exists_valuation_world;
-  use (λ w a => match a with | 0 => y ≺ w | 1 => w = y | _ => False), x;
-  suffices x ≺ y ∧ ∃ z, x ≺ z ∧ (∀ u, z ≺ u → ¬y ≺ u) ∧ ¬z = y by
-    simpa [Satisfies, Semantics.Realize];
-  refine ⟨Rxy, z, Rxz, ?_, by tauto⟩;
-  . intro u;
-    contrapose;
-    push_neg;
-    intro Ryu;
-    exact hu u Ryu;
+lemma isPiecewiseConvergent_of_validate_axiomWeakPoint2 (h : F ⊧ (Axioms.WeakPoint2 (.atom 0) (.atom 1))) : F.IsPiecewiseConvergent where
+  p_convergent := by
+    dsimp [PiecewiseConvergent];
+    revert h;
+    contrapose!;
+    rintro ⟨x, y, z, Rxy, Rxz, nyz, hu⟩;
+    apply ValidOnFrame.not_of_exists_valuation_world;
+    use (λ w a => match a with | 0 => y ≺ w | 1 => w = y | _ => False), x;
+    suffices x ≺ y ∧ ∃ z, x ≺ z ∧ (∀ u, z ≺ u → ¬y ≺ u) ∧ ¬z = y by
+      simpa [Satisfies, Semantics.Realize];
+    refine ⟨Rxy, z, Rxz, ?_, by tauto⟩;
+    . intro u;
+      contrapose;
+      push_neg;
+      intro Ryu;
+      exact hu u Ryu;
 
 end definability
 
@@ -59,45 +73,40 @@ open Formula.Kripke
 open MaximalConsistentTableau
 open canonicalModel
 
-namespace Canonical
+instance [Entailment.HasAxiomWeakPoint2 𝓢] : (canonicalFrame 𝓢).IsPiecewiseConvergent where
+  p_convergent := by
+    rintro x y z Rxy Rxz eyz;
+    have ⟨u, hu⟩ := lindenbaum (𝓢 := 𝓢) (t₀ := ⟨y.1.1.prebox, z.1.2.predia⟩) $ by
+      rintro Γ Δ hΓ hΔ;
+      by_contra hC;
+      have hγ : □(Γ.conj) ∈ y.1.1 := y.mdp_mem₁_provable collect_box_fconj! $ iff_mem₁_fconj.mpr (by simpa using hΓ);
+      have hδ : ◇(Δ.disj) ∈ z.1.2 := mdp_mem₂_provable distribute_dia_fdisj! $ iff_mem₂_fdisj.mpr (by simpa using hΔ);
+      generalize Γ.conj = γ₁ at hγ hC;
+      generalize Δ.disj = δ₁ at hδ hC;
+      obtain ⟨δ₂, hδ₂₁, hδ₂₂⟩ := exists₁₂_of_ne eyz;
 
-instance [Entailment.HasAxiomWeakPoint2 𝓢] : IsWeakConfluent _ (canonicalFrame 𝓢).Rel := ⟨by
-  rintro x y z ⟨Rxy, Rxz, eyz⟩;
-  have ⟨u, hu⟩ := lindenbaum (𝓢 := 𝓢) (t₀ := ⟨y.1.1.prebox, z.1.2.predia⟩) $ by
-    rintro Γ Δ hΓ hΔ;
-    by_contra hC;
-    have hγ : □(Γ.conj) ∈ y.1.1 := y.mdp_mem₁_provable collect_box_fconj! $ iff_mem₁_fconj.mpr (by simpa using hΓ);
-    have hδ : ◇(Δ.disj) ∈ z.1.2 := mdp_mem₂_provable distribute_dia_fdisj! $ iff_mem₂_fdisj.mpr (by simpa using hΔ);
-    generalize Γ.conj = γ₁ at hγ hC;
-    generalize Δ.disj = δ₁ at hδ hC;
-    obtain ⟨δ₂, hδ₂₁, hδ₂₂⟩ := exists₁₂_of_ne eyz;
-
-    have : 𝓢 ⊢! □γ₁ ➝ □δ₁ := imply_box_distribute'! hC;
-    have : 𝓢 ⊢! □γ₁ ⋏ δ₂ ➝ □δ₁ ⋏ δ₂ := CKK!_of_C! this;
-    have : □δ₁ ⋏ δ₂ ∈ y.1.1 := mdp_mem₁_provable this $ by
-      apply iff_mem₁_and.mpr; constructor <;> assumption;
-    have : ◇(□δ₁ ⋏ δ₂) ∈ x.1.1 := def_rel_dia_mem₁.mp Rxy this;
-    have : □(◇δ₁ ⋎ δ₂) ∈ x.1.1 := mdp_mem₁_provable axiomWeakPoint2! this;
-    have : ◇δ₁ ⋎ δ₂ ∈ z.1.1 := def_rel_box_mem₁.mp Rxz this;
-    rcases iff_mem₁_or.mp this with (hδ₁ | hδ₂);
-    . have : ◇δ₁ ∉ z.1.2 := iff_not_mem₂_mem₁.mpr hδ₁;
-      contradiction;
-    . have : δ₂ ∉ z.1.2 := iff_not_mem₂_mem₁.mpr hδ₂;
-      contradiction;
-  use u;
-  constructor;
-  . apply def_rel_box_mem₁.mpr;
-    intro φ hφ;
-    apply hu.1 hφ;
-  . apply def_rel_dia_mem₂.mpr;
-    intro φ hφ;
-    apply hu.2 hφ;
-⟩
-
-end Canonical
+      have : 𝓢 ⊢! □γ₁ ➝ □δ₁ := imply_box_distribute'! hC;
+      have : 𝓢 ⊢! □γ₁ ⋏ δ₂ ➝ □δ₁ ⋏ δ₂ := CKK!_of_C! this;
+      have : □δ₁ ⋏ δ₂ ∈ y.1.1 := mdp_mem₁_provable this $ by
+        apply iff_mem₁_and.mpr; constructor <;> assumption;
+      have : ◇(□δ₁ ⋏ δ₂) ∈ x.1.1 := def_rel_dia_mem₁.mp Rxy this;
+      have : □(◇δ₁ ⋎ δ₂) ∈ x.1.1 := mdp_mem₁_provable axiomWeakPoint2! this;
+      have : ◇δ₁ ⋎ δ₂ ∈ z.1.1 := def_rel_box_mem₁.mp Rxz this;
+      rcases iff_mem₁_or.mp this with (hδ₁ | hδ₂);
+      . have : ◇δ₁ ∉ z.1.2 := iff_not_mem₂_mem₁.mpr hδ₁;
+        contradiction;
+      . have : δ₂ ∉ z.1.2 := iff_not_mem₂_mem₁.mpr hδ₂;
+        contradiction;
+    use u;
+    constructor;
+    . apply def_rel_box_mem₁.mpr;
+      intro φ hφ;
+      apply hu.1 hφ;
+    . apply def_rel_dia_mem₂.mpr;
+      intro φ hφ;
+      apply hu.2 hφ;
 
 end canonicality
-
 
 end Kripke
 
