Foundation/Modal/Kripke/AxiomWeakPoint3.lean
@@ -1,20 +1,29 @@
 import Foundation.Modal.Kripke.Completeness
-
+import Foundation.Vorspiel.HRel.Connected
 
 namespace LO.Modal
 
 namespace Kripke
 
-open Formula.Kripke
 
-instance : IsWeakConnected _ whitepoint.Rel := ⟨by tauto⟩
+variable {F : Kripke.Frame}
+
+namespace Frame
+
+class IsPiecewiseConnected (F : Frame) extends _root_.IsPiecewiseConnected F.Rel
+
+end Frame
+
+instance : whitepoint.IsPiecewiseConnected where
+  p_connected := by tauto
 
 
 section definability
 
-variable {F : Kripke.Frame}
+open Formula (atom)
+open Formula.Kripke
 
-lemma validate_WeakPoint3_of_weakConnected [IsWeakConnected _ F] : F ⊧ (Axioms.WeakPoint3 (.atom 0) (.atom 1)) := by
+lemma validate_WeakPoint3_of_weakConnected [F.IsPiecewiseConnected] : F ⊧ (Axioms.WeakPoint3 (.atom 0) (.atom 1)) := by
   rintro V x;
   apply Satisfies.or_def.mpr;
   suffices
@@ -28,22 +37,24 @@ lemma validate_WeakPoint3_of_weakConnected [IsWeakConnected _ F] : F ⊧ (Axioms
     by_contra hC;
     subst hC;
     contradiction;
-  rcases IsWeakConnected.weak_connected ⟨Rxy, Rxz, nyz⟩ with (Ryz | Rzy);
+  rcases IsPiecewiseConnected.p_connected' Rxy Rxz nyz with (Ryz | Rzy);
   . apply nhz0; exact hz _ Ryz;
   . apply nhy1; exact hy _ Rzy;
 
-lemma weakConnected_of_validate_WeakPoint3 : F ⊧ (Axioms.WeakPoint3 (.atom 0) (.atom 1)) → WeakConnected F := by
-  contrapose;
-  intro hCon;
-  obtain ⟨x, y, Rxy, z, Rxz, nyz, nRyz, nRzy⟩ := by simpa [WeakConnected] using hCon;
-  apply ValidOnFrame.not_of_exists_valuation_world;
-  use (λ w a => match a with | 0 => w = y ∨ y ≺ w | 1 => w = z ∨ z ≺ w | _ => True), x;
-  suffices
-    ∃ w, x ≺ w ∧ (w = y ∨ y ≺ w) ∧ (∀ (v : F.World), w ≺ v → ¬v = y → y ≺ v) ∧ ¬w = z ∧ ¬z ≺ w ∧
-    ∃ w, x ≺ w ∧ (w = z ∨ z ≺ w) ∧ (∀ (v : F.World), w ≺ v → ¬v = z → z ≺ v) ∧ ¬w = y ∧ ¬y ≺ w by
-    simpa [Semantics.Realize, Satisfies];
-  refine ⟨y, Rxy, ?_, ?_, ?_, ?_, z, Rxz, ?_, ?_, ?_, ?_⟩;
-  all_goals tauto;
+lemma isPiecewiseConnected_of_validate_axiomWeakPoint3 (h : F ⊧ (Axioms.WeakPoint3 (.atom 0) (.atom 1))) : F.IsPiecewiseConnected where
+  p_connected := by
+    dsimp [PiecewiseConnected];
+    revert h;
+    contrapose!;
+    rintro ⟨x, y, z, Rxy, Rxz, nRyz, nyz, nRzy⟩;
+    apply ValidOnFrame.not_of_exists_valuation_world;
+    use (λ w a => match a with | 0 => w = y ∨ y ≺ w | 1 => w = z ∨ z ≺ w | _ => True), x;
+    suffices
+      ∃ w, x ≺ w ∧ (w = y ∨ y ≺ w) ∧ (∀ (v : F.World), w ≺ v → ¬v = y → y ≺ v) ∧ ¬w = z ∧ ¬z ≺ w ∧
+      ∃ w, x ≺ w ∧ (w = z ∨ z ≺ w) ∧ (∀ (v : F.World), w ≺ v → ¬v = z → z ≺ v) ∧ ¬w = y ∧ ¬y ≺ w by
+      simpa [Semantics.Realize, Satisfies];
+    refine ⟨y, Rxy, ?_, ?_, ?_, ?_, z, Rxz, ?_, ?_, ?_, ?_⟩;
+    all_goals tauto;
 
 end definability
 
@@ -58,70 +69,65 @@ open Entailment
 open MaximalConsistentTableau
 open canonicalModel
 
-namespace Canonical
+instance [Entailment.HasAxiomWeakPoint3 𝓢] : (canonicalFrame 𝓢).IsPiecewiseConnected where
+  p_connected := by
+    rintro x y z Rxy Rxz;
+    by_contra! hC;
+    rcases hC with ⟨nRyz, neyz, nRzy⟩;
 
-instance [Entailment.HasAxiomWeakPoint3 𝓢] : IsWeakConnected _ (canonicalFrame 𝓢).Rel := ⟨by
-  rintro x y z ⟨Rxy, Rxz, eyz⟩;
-  by_contra hC;
-  push_neg at hC;
-  rcases hC with ⟨nRyz, nRzy⟩;
+    obtain ⟨φ₁, hφ₁y, hφ₁z⟩ := Set.not_subset.mp nRyz;
+    replace hφ₁y : □φ₁ ∈ y.1.1 := by simpa using hφ₁y;
+    replace hφ₁z : φ₁ ∈ z.1.2 := iff_not_mem₁_mem₂.mp hφ₁z;
+    obtain ⟨φ₂, hφ₂y, hφ₂z⟩ := exists₁₂_of_ne neyz;
+    let φ := φ₁ ⋎ φ₂;
 
-  obtain ⟨φ₁, hφ₁y, hφ₁z⟩ := Set.not_subset.mp nRyz;
-  replace hφ₁y : □φ₁ ∈ y.1.1 := by simpa using hφ₁y;
-  replace hφ₁z : φ₁ ∈ z.1.2 := iff_not_mem₁_mem₂.mp hφ₁z;
-  obtain ⟨φ₂, hφ₂y, hφ₂z⟩ := exists₁₂_of_ne eyz;
-  let φ := φ₁ ⋎ φ₂;
+    obtain ⟨ψ₁, hψz, hψy⟩ := Set.not_subset.mp nRzy;
+    replace hψ₁z : □ψ₁ ∈ z.1.1 := by simpa using hψz;
+    replace hψ₁y : ψ₁ ∈ y.1.2 := iff_not_mem₁_mem₂.mp hψy;
+    obtain ⟨ψ₂, hψ₂z, hψ₂y⟩ := exists₂₁_of_ne neyz;
+    let ψ := ψ₁ ⋎ ψ₂;
 
-  obtain ⟨ψ₁, hψz, hψy⟩ := Set.not_subset.mp nRzy;
-  replace hψ₁z : □ψ₁ ∈ z.1.1 := by simpa using hψz;
-  replace hψ₁y : ψ₁ ∈ y.1.2 := iff_not_mem₁_mem₂.mp hψy;
-  obtain ⟨ψ₂, hψ₂z, hψ₂y⟩ := exists₂₁_of_ne eyz;
-  let ψ := ψ₁ ⋎ ψ₂;
-
-  apply x.neither (φ := □(⊡φ ➝ ψ) ⋎ □(⊡ψ ➝ φ));
-  constructor;
-  . exact iff_provable_mem₁.mp axiomWeakPoint3! x;
-  . apply iff_mem₂_or.mpr;
+    apply x.neither (φ := □(⊡φ ➝ ψ) ⋎ □(⊡ψ ➝ φ));
     constructor;
-    . apply iff_mem₂_box.mpr;
-      use y;
+    . exact iff_provable_mem₁.mp axiomWeakPoint3! x;
+    . apply iff_mem₂_or.mpr;
       constructor;
-      . assumption;
-      . apply iff_mem₂_imp.mpr;
+      . apply iff_mem₂_box.mpr;
+        use y;
         constructor;
-        . apply iff_mem₁_and.mpr;
+        . assumption;
+        . apply iff_mem₂_imp.mpr;
           constructor;
-          . apply iff_mem₁_or.mpr; tauto;
-          . apply iff_mem₁_box.mpr
-            intro u Ryu;
-            apply iff_mem₁_or.mpr;
-            left;
-            exact Ryu hφ₁y;
-        . apply iff_mem₂_or.mpr;
-          constructor;
-          . assumption;
-          . assumption;
-    . apply iff_mem₂_box.mpr;
-      use z;
-      constructor;
-      . assumption;
-      . apply iff_mem₂_imp.mpr;
+          . apply iff_mem₁_and.mpr;
+            constructor;
+            . apply iff_mem₁_or.mpr; tauto;
+            . apply iff_mem₁_box.mpr
+              intro u Ryu;
+              apply iff_mem₁_or.mpr;
+              left;
+              exact Ryu hφ₁y;
+          . apply iff_mem₂_or.mpr;
+            constructor;
+            . assumption;
+            . assumption;
+      . apply iff_mem₂_box.mpr;
+        use z;
         constructor;
-        . apply iff_mem₁_and.mpr;
+        . assumption;
+        . apply iff_mem₂_imp.mpr;
           constructor;
-          . apply iff_mem₁_or.mpr; tauto;
-          . apply iff_mem₁_box.mpr
-            intro u Rzu;
-            apply iff_mem₁_or.mpr;
-            left;
-            exact Rzu hψ₁z;
-        . apply iff_mem₂_or.mpr;
-          constructor;
-          . assumption;
-          . assumption;
-⟩
-
-end Canonical
+          . apply iff_mem₁_and.mpr;
+            constructor;
+            . apply iff_mem₁_or.mpr; tauto;
+            . apply iff_mem₁_box.mpr
+              intro u Rzu;
+              apply iff_mem₁_or.mpr;
+              left;
+              exact Rzu hψ₁z;
+          . apply iff_mem₂_or.mpr;
+            constructor;
+            . assumption;
+            . assumption;
 
 end canonicality
 
