Foundation/Vorspiel/HRel/Connected.lean
@@ -5,7 +5,10 @@ variable {α} {R : HRel α}
 def PiecewiseConnected (R : HRel α) := ∀ ⦃x y z⦄, R x y → R x z → (R y z ∨ y = z ∨ R z y)
 
 class IsPiecewiseConnected (R : HRel α) where
-  pconnected : PiecewiseConnected R
+  p_connected : PiecewiseConnected R
+
+lemma IsPiecewiseConnected.p_connected' {R : HRel α} [IsPiecewiseConnected R] {x y z : α} (Rxy : R x y) (Rxz : R x z) (hyz : y ≠ z) : R y z ∨ R z y := by
+  rcases IsPiecewiseConnected.p_connected Rxy Rxz with (Ryz | rfl | Rzy) <;> tauto;
 
 instance [IsTrichotomous _ R] : IsPiecewiseConnected R :=
   ⟨fun ⦃_ y z⦄ _ _ ↦ IsTrichotomous.trichotomous y z⟩
@@ -14,13 +17,13 @@ instance [IsTrichotomous _ R] : IsPiecewiseConnected R :=
 def PiecewiseStronglyConnected (R : HRel α) := ∀ ⦃x y z⦄, R x y → R x z → (R y z ∨ R z y)
 
 class IsPiecewiseStronglyConnected (R : HRel α) where
-  psconnected : PiecewiseStronglyConnected R
+  ps_connected : PiecewiseStronglyConnected R
 
 instance [IsTotal _ R] : IsPiecewiseStronglyConnected R := ⟨fun ⦃_ y z⦄ _ _ ↦ IsTotal.total y z⟩
 
 instance [IsPiecewiseConnected R] [IsRefl _ R] : IsPiecewiseStronglyConnected R := ⟨by
   intro x y z Rxy Rxz;
-  rcases IsPiecewiseConnected.pconnected Rxy Rxz with (Ryz | rfl | Rzy);
+  rcases IsPiecewiseConnected.p_connected Rxy Rxz with (Ryz | rfl | Rzy);
   . tauto;
   . left; apply refl;
   . tauto;
@@ -28,5 +31,5 @@ instance [IsPiecewiseConnected R] [IsRefl _ R] : IsPiecewiseStronglyConnected R 
 
 instance [IsPiecewiseStronglyConnected R] : IsPiecewiseConnected R := ⟨by
   intro x y z Rxy Rxz;
-  rcases IsPiecewiseStronglyConnected.psconnected Rxy Rxz <;> tauto;
+  rcases IsPiecewiseStronglyConnected.ps_connected Rxy Rxz <;> tauto;
 ⟩
