Foundation/Modal/Kripke/AxiomGrz.lean
@@ -17,7 +17,7 @@ open Relation (IrreflGen)
 variable {F : Kripke.Frame}
 
 lemma validate_AxiomGrz_of_refl_trans_wcwf
-  [IsRefl _ F.Rel]
+  [F.IsReflexive.Rel]
   [F.IsTransitive.Rel]
   [IsWeaklyConverseWellFounded _ F.Rel]
   : F ⊧ (Axioms.Grz (.atom 0)) := by
