Foundation/Propositional/Kripke/Logic/Cl.lean
@@ -11,7 +11,7 @@ open Formula.Kripke
 namespace Kripke.FrameClass
 
 protected abbrev euclidean : FrameClass := { F | F.IsEuclidean }
-protected abbrev finite_symmetric : FrameClass := { F | Finite F ∧ IsSymm _ F }
+protected abbrev finite_symmetric : FrameClass := { F | Finite F ∧ F.IsSymmetric }
 protected abbrev finite_euclidean : FrameClass := { F | Finite F ∧ F.IsEuclidean }
 
 lemma eq_finite_euclidean_finite_symmetric : FrameClass.finite_euclidean = FrameClass.finite_symmetric := by
